---
layout:    zh_post
Topic:     线性代数
Title:     重要线性变换
Revised:   2018-04-29 17:00:00 +08 @ 中国-新疆-乌鲁木齐 +06
Authors:   璀璨星辰
Resources:
---

> ### 函数的线性变换

> $$
> \begin{alignedat}{3}
> \fbox{1}\; & f (x) \xlongequal[x \in \lbrack \alpha, \beta \rbrack; t \in \lbrack 0, 1 \rbrack]{x = \alpha + (\beta - \alpha) t} f (\alpha + (\beta - \alpha) t) \\
> \fbox{2}\; & f (t + T) = f (t) \xlongequal[f \left( \frac{T}{2 \pi} x \right)]{t = \frac{T}{2 \pi} x} g (x) = g (x + 2 \pi) \\
> \fbox{3}\; & g (x) \xlongequal[g (\beta) = f (\beta)]{g (\alpha) = f (\alpha)} f (\alpha) + \dfrac{f (\beta) - f (\alpha)}{\beta - \alpha} (x - \alpha) \\
> \end{alignedat}
> $$
>

