```
# 典型的命题逻辑等价定律，共35行
# 常值，共4行
[消去律] 0 ⇔ P ∧ 0
[完全律] 1 ⇔ P ∨ 1
[矛盾律] 0 ⇔ P ∧ ¬P
[枚举律] 1 ⇔ P ∨ ¬P

# 单项，共7行
[双否律] P ⇔ ¬¬P
[缩减律] P ⇔ P ∧ 1
[扩充律] P ⇔ P ∨ 0
[幂等律] P ⇔ P ∧ P
[幂等律] P ⇔ P ∨ P
[公约律] P ⇔ P ∧ (P ∨ Q)
[公倍律] P ⇔ P ∨ (P ∧ Q)

# 与或，共4行
[交换律]    P ∧ Q ⇔  Q ∧ P
[交换律]    P ∨ Q ⇔  Q ∨ P
[置否律] ¬(P ∧ Q) ⇔ ¬P ∨ ¬Q
[置否律] ¬(P ∨ Q) ⇔ ¬P ∧ ¬Q

# 推理，共5行
[善意律] P → Q ⇔ ¬P ∨ Q
[逆否法] P → Q ⇔ ¬Q → ¬P
[交换律] P ↔ Q ⇔  Q ↔ P
[逆否法] P ↔ Q ⇔ ¬P ↔ ¬Q
[双向律] P ↔ Q ⇔ (P → Q) ∧ (Q → P)

# 电路，共5行
[与非律] P ↑ Q ⇔ ¬(P ∧ Q)
[或非律] P ↓ Q ⇔ ¬(P ∨ Q)
[异或律] P ⊕ Q ⇔ ¬(P ↔ Q)
[异或律] P ⊕ Q ⇔  ¬P ↔ Q
[异或律] P ⊕ Q ⇔  (P ∨ Q) ∧ ¬(P ∧ Q)

# 定律，共4行
[结合律] P ∧ (Q ∧ R) ⇔ (P ∧ Q) ∧ R
[结合律] P ∨ (Q ∨ R) ⇔ (P ∨ Q) ∨ R
[分配律] P ∧ (Q ∨ R) ⇔ (P ∧ Q) ∨ (P ∧ R)
[分配律] P ∨ (Q ∧ R) ⇔ (P ∨ Q) ∧ (P ∨ R)

# 方法，共6行
[归谬法] (P → Q) ∧ (P → ¬Q) ⇔ ¬P
[归论法] (¬P → Q) ∧ (P → Q) ⇔ Q
[反证法]              P → Q ⇔ ¬(P ∧ ¬Q)
[附加法]        P → (Q → R) ⇔ (P ∧ Q) → R
[分治法]        (P ∨ Q) → R ⇔ (P → R) ∧ (Q → R)
[循环法]  (P ↔ Q) ∧ (Q ↔ R) ⇔ (P → Q) ∧ (Q → R) ∧ (R → P)

# 典型的命题逻辑演绎定律，共20行
[附加结论]                            P  ⇒ P ∨ Q
[善意推断]                           ¬P  ⇒ P → Q
[善意推断]                            Q  ⇒ P → Q
[简化前提]                        P ∧ Q  ⇒ P
[善意推断]                      ¬(P → Q) ⇒ P
[善意推断]                      ¬(P → Q) ⇒ ¬Q
[排挤妨碍]                   P ∧ (Q ∨ R) ⇒ Q ∨ (P ∧ R)
[排除矛盾]                  ¬P ∧ (P ∨ Q) ⇒ Q
[排除矛盾]                  ¬P ∨ (P ∧ Q) ⇒ Q
[已知前提]                   P ∧ (P → Q) ⇒ Q
[结论谬误]                  ¬Q ∧ (P → Q) ⇒ ¬P
[合取演绎]             (P ∧ Q) ∧ (Q → R) ⇒ P ∧ R
[析取演绎]             (P ∨ Q) ∧ (Q → R) ⇒ P ∨ R
[三段等价]             (P ↔ Q) ∧ (Q ↔ R) ⇒ P ↔ R
[三段演绎]             (P → Q) ∧ (Q → R) ⇒ P → R
[归并演绎]             (P ∨ R) → (Q ∧ S) ⇒ (P → Q) ∧ (R → S)
[归并演绎]             (P → Q) ∧ (R → S) ⇒ (P ∨ R) → (Q ∨ S) ⇒ (P ∧ R) → (Q ∨ S)
                                         ⇒ (P ∧ R) → (Q ∧ S)
[二择前提]   (P ∨ R) ∧ (P → Q) ∧ (R → S) ⇒ Q ∨ S
[结论二难] (¬Q ∨ ¬S) ∧ (P → Q) ∧ (R → S) ⇒ ¬P ∨ ¬R
```

| 命题 | 命题 | 命题 | 命题 |      复合命题①      |      复合命题②      |      复合命题③      |      复合命题④      |      复合命题⑤      |
| :--: | :--: | :--: | :--: | :-----------------: | :-----------------: | :-----------------: | :-----------------: | :-----------------: |
|  P   |  Q   |  R   |  S   | [(P ∨ R) → (Q ∧ S)] | [(P → Q) ∧ (R → S)] | [(P ∨ R) → (Q ∨ S)] | [(P ∧ R) → (Q ∧ S)] | [(P ∧ R) → (Q ∨ S)] |
|  真  |  真  |  真  |  真  |   [真 → 真] = 真    |   [真 ∧ 真] = 真    |   [真 → 真] = 真    |   [真 → 真] = 真    |   [真 → 真] = 真    |
|  真  |  真  |  假  |  真  |   [真 → 真] = 真    |   [真 ∧ 真] = 真    |   [真 → 真] = 真    |   [假 → 真] = 真    |   [假 → 真] = 真    |
|  真  |  假  |  真  |  真  |   [真 → 假] = 假    |   [假 ∧ 真] = 假    |   [真 → 真] = 真    |   [真 → 假] = 假    |   [真 → 真] = 真    |
|  真  |  假  |  假  |  真  |   [真 → 假] = 假    |   [假 ∧ 真] = 假    |   [真 → 真] = 真    |   [假 → 假] = 真    |   [假 → 真] = 真    |
|  假  |  真  |  真  |  真  |   [真 → 真] = 真    |   [真 ∧ 真] = 真    |   [真 → 真] = 真    |   [假 → 真] = 真    |   [假 → 真] = 真    |
|  假  |  真  |  假  |  真  |   [假 → 真] = 真    |   [真 ∧ 真] = 真    |   [假 → 真] = 真    |   [假 → 真] = 真    |   [假 → 真] = 真    |
|  假  |  假  |  真  |  真  |   [真 → 假] = 假    |   [真 ∧ 真] = 真    |   [真 → 真] = 真    |   [假 → 假] = 真    |   [假 → 真] = 真    |
|  假  |  假  |  假  |  真  |   [假 → 假] = 真    |   [真 ∧ 真] = 真    |   [假 → 真] = 真    |   [假 → 假] = 真    |   [假 → 真] = 真    |
|      |      |      |      |                     |                     |                     |                     |                     |
|  真  |  真  |  真  |  假  |   [真 → 假] = 假    |   [真 ∧ 假] = 假    |   [真 → 真] = 真    |   [真 → 假] = 假    |   [真 → 真] = 真    |
|  真  |  真  |  假  |  假  |   [真 → 假] = 假    |   [真 ∧ 真] = 真    |   [真 → 真] = 真    |   [假 → 假] = 真    |   [假 → 真] = 真    |
|  真  |  假  |  真  |  假  |   [真 → 假] = 假    |   [假 ∧ 假] = 假    |   [真 → 假] = 假    |   [真 → 假] = 假    |   [真 → 假] = 假    |
|  真  |  假  |  假  |  假  |   [真 → 假] = 假    |   [假 ∧ 真] = 假    |   [真 → 假] = 假    |   [假 → 假] = 真    |   [假 → 假] = 真    |
|  假  |  真  |  真  |  假  |   [真 → 假] = 假    |   [真 ∧ 假] = 假    |   [真 → 真] = 真    |   [假 → 假] = 真    |   [假 → 真] = 真    |
|  假  |  真  |  假  |  假  |   [假 → 假] = 真    |   [真 ∧ 真] = 真    |   [假 → 真] = 真    |   [假 → 假] = 真    |   [假 → 真] = 真    |
|  假  |  假  |  真  |  假  |   [真 → 假] = 假    |   [真 ∧ 假] = 假    |   [真 → 假] = 假    |   [假 → 假] = 真    |   [假 → 假] = 真    |
|  假  |  假  |  假  |  假  |   [假 → 假] = 真    |   [真 ∧ 真] = 真    |   [假 → 假] = 真    |   [假 → 假] = 真    |   [假 → 假] = 真    |
|      |      |      |      |        ① ⇒ ②        |        ② ⇒ ③        |        ③ ⇒ ⑤        |        ④ ⇒ ⑤        |                     |
|      |      |      |      |                     |        ② ⇒ ④        |                     |                     |                     |

| 命题 | 命题 | 命题 | 命题 |           排挤妨碍            |           合取演绎            |           析取演绎            |           三段等价            |           三段演绎            |                 归并演绎                  |                二择前提                 |                  结论二难                   |
| :--: | :--: | :--: | :--: | :---------------------------: | :---------------------------: | :---------------------------: | :---------------------------: | :---------------------------: | :---------------------------------------: | :-------------------------------------: | :-----------------------------------------: |
|  P   |  Q   |  R   |  S   | [P ∧ (Q ∨ R)] → [Q ∨ (P ∧ R)] | [(P ∧ Q) ∧ (Q → R)] → [P ∧ R] | [(P ∨ Q) ∧ (Q → R)] → [P ∨ R] | [(P ↔ Q) ∧ (Q ↔ R)] ↔ [P ↔ R] | [(P ↔ Q) ∧ (Q ↔ R)] → [P ↔ R] | [(P ∨ R) → (Q ∧ S)] → [(P → Q) ∧ (R → S)] | [(P ∨ R) ∧ (P → Q) ∧ (R → S)] → [Q ∨ S] | [(¬Q ∨ ¬S) ∧ (P → Q) ∧ (R → S)] → [¬P ∨ ¬R] |
|  真  |  真  |  真  |  真  |  [真 ∧ 真] → [真 ∨ 真] = 真   |      [真 ∧ 真] → 真 = 真      |      [真 ∧ 真] → 真 = 真      |      [真 ∧ 真] ↔ 真 = 真      |      [真 ∧ 真] → 真 = 真      |        [真 → 真] → [真 ∧ 真] = 真         |        [真 ∧ 真 ∧ 真] → 真 = 真         |          [假 ∧ 真 ∧ 真] → 假 = 真           |
|  真  |  真  |  假  |  真  |  [真 ∧ 真] → [真 ∨ 假] = 真   |      [真 ∧ 假] → 假 = 真      |      [真 ∧ 假] → 真 = 真      |      [真 ∧ 假] ↔ 假 = 真      |      [真 ∧ 假] → 假 = 真      |        [真 → 真] → [真 ∧ 真] = 真         |        [真 ∧ 真 ∧ 真] → 真 = 真         |          [假 ∧ 真 ∧ 真] → 真 = 真           |
|  真  |  假  |  真  |  真  |  [真 ∧ 真] → [假 ∨ 真] = 真   |      [假 ∧ 真] → 真 = 真      |      [真 ∧ 真] → 真 = 真      |      [假 ∧ 假] ↔ 真 = 假      |      [假 ∧ 假] → 真 = 真      |        [真 → 假] → [假 ∧ 真] = 真         |        [真 ∧ 假 ∧ 真] → 真 = 真         |          [真 ∧ 假 ∧ 真] → 假 = 真           |
|  真  |  假  |  假  |  真  |  [真 ∧ 假] → [假 ∨ 假] = 真   |      [假 ∧ 真] → 假 = 真      |      [真 ∧ 真] → 真 = 真      |      [假 ∧ 真] ↔ 假 = 真      |      [假 ∧ 真] → 假 = 真      |        [真 → 假] → [假 ∧ 真] = 真         |        [真 ∧ 假 ∧ 真] → 真 = 真         |          [真 ∧ 假 ∧ 真] → 真 = 真           |
|  假  |  真  |  真  |  真  |  [假 ∧ 真] → [真 ∨ 假] = 真   |      [假 ∧ 真] → 假 = 真      |      [真 ∧ 真] → 真 = 真      |      [假 ∧ 真] ↔ 假 = 真      |      [假 ∧ 真] → 假 = 真      |        [真 → 真] → [真 ∧ 真] = 真         |        [真 ∧ 真 ∧ 真] → 真 = 真         |          [假 ∧ 真 ∧ 真] → 真 = 真           |
|  假  |  真  |  假  |  真  |  [假 ∧ 真] → [真 ∨ 假] = 真   |      [假 ∧ 假] → 假 = 真      |      [真 ∧ 假] → 假 = 真      |      [假 ∧ 假] ↔ 真 = 假      |      [假 ∧ 假] → 真 = 真      |        [假 → 真] → [真 ∧ 真] = 真         |        [假 ∧ 真 ∧ 真] → 真 = 真         |          [假 ∧ 真 ∧ 真] → 真 = 真           |
|  假  |  假  |  真  |  真  |  [假 ∧ 真] → [假 ∨ 假] = 真   |      [假 ∧ 真] → 假 = 真      |      [假 ∧ 真] → 真 = 真      |      [真 ∧ 假] ↔ 假 = 真      |      [真 ∧ 假] → 假 = 真      |        [真 → 假] → [真 ∧ 真] = 真         |        [真 ∧ 真 ∧ 真] → 真 = 真         |          [真 ∧ 真 ∧ 真] → 真 = 真           |
|  假  |  假  |  假  |  真  |  [假 ∧ 假] → [假 ∨ 假] = 真   |      [假 ∧ 真] → 假 = 真      |      [假 ∧ 真] → 假 = 真      |      [真 ∧ 真] ↔ 真 = 真      |      [真 ∧ 真] → 真 = 真      |        [假 → 假] → [真 ∧ 真] = 真         |        [假 ∧ 真 ∧ 真] → 真 = 真         |          [真 ∧ 真 ∧ 真] → 真 = 真           |
|      |      |      |      |   P ∧ (Q ∨ R) ⇒ Q ∨ (P ∧ R)   |   (P ∧ Q) ∧ (Q → R) ⇒ P ∧ R   |   (P ∨ Q) ∧ (Q → R) ⇒ P ∨ R   |   (P ↔ Q) ∧ (Q ↔ R) ⇒ P ↔ R   |   (P ↔ Q) ∧ (Q ↔ R) ⇒ P ↔ R   |                                           |                                         |                                             |
|  真  |  真  |  真  |  假  |                               |                               |                               |   (P ↔ Q) ∧ (Q ↔ R) ⇎ P ↔ R   |                               |        [真 → 假] → [真 ∧ 假] = 真         |        [真 ∧ 真 ∧ 假] → 真 = 真         |          [真 ∧ 真 ∧ 假] → 假 = 真           |
|  真  |  真  |  假  |  假  |                               |                               |                               |                               |                               |        [真 → 假] → [真 ∧ 真] = 真         |        [真 ∧ 真 ∧ 真] → 真 = 真         |          [真 ∧ 真 ∧ 真] → 真 = 真           |
|  真  |  假  |  真  |  假  |                               |                               |                               |                               |                               |        [真 → 假] → [假 ∧ 假] = 真         |        [真 ∧ 假 ∧ 假] → 假 = 真         |          [真 ∧ 假 ∧ 假] → 假 = 真           |
|  真  |  假  |  假  |  假  |                               |                               |                               |                               |                               |        [真 → 假] → [假 ∧ 真] = 真         |        [真 ∧ 假 ∧ 真] → 假 = 真         |          [真 ∧ 假 ∧ 真] → 真 = 真           |
|  假  |  真  |  真  |  假  |                               |                               |                               |                               |                               |        [真 → 假] → [真 ∧ 假] = 真         |        [真 ∧ 真 ∧ 假] → 真 = 真         |          [真 ∧ 真 ∧ 假] → 真 = 真           |
|  假  |  真  |  假  |  假  |                               |                               |                               |                               |                               |        [假 → 假] → [真 ∧ 真] = 真         |        [假 ∧ 真 ∧ 真] → 真 = 真         |          [真 ∧ 真 ∧ 真] → 真 = 真           |
|  假  |  假  |  真  |  假  |                               |                               |                               |                               |                               |        [真 → 假] → [真 ∧ 假] = 真         |        [真 ∧ 真 ∧ 假] → 假 = 真         |          [真 ∧ 真 ∧ 假] → 真 = 真           |
|  假  |  假  |  假  |  假  |                               |                               |                               |                               |                               |        [假 → 假] → [真 ∧ 真] = 真         |        [假 ∧ 真 ∧ 真] → 假 = 真         |          [真 ∧ 真 ∧ 真] → 真 = 真           |
|      |      |      |      |                               |                               |                               |                               |                               |   (P ∨ R) → (Q ∧ S) ⇒ (P → Q) ∧ (R → S)   |   (P ∨ R) ∧ (P → Q) ∧ (R → S) ⇒ Q ∨ S   |   (¬Q ∨ ¬S) ∧ (P → Q) ∧ (R → S) ⇒ ¬P ∨ ¬R   |